theories/Sem/Call.v
@@ -1,0 +1,72 @@
+(*
+ * Copyright (C) BedRock Systems Inc. 2019 Gregory Malecha
+ *
+ * SPDX-License-Identifier:AGPL-3.0-or-later
+ *)
+Require Import Coq.ZArith.ZArith.
+Require Import Coq.Lists.List.
+Require Import Coq.Strings.String.
+
+Local Open Scope string_scope.
+Local Open Scope Z_scope.
+
+From Cpp Require Import
+     Ast.
+From Cpp.Sem Require Import
+     ChargeUtil Logic PLogic Semantics Wp.
+
+Module Type Call.
+
+  Section with_resolve.
+    Context {resolve : genv}.
+    Variable ti : thread_info.
+    Variable ρ : region.
+
+    Local Notation wp := (wp (resolve:=resolve)  ti ρ).
+    Local Notation wpe := (wpe (resolve:=resolve) ti ρ).
+    Local Notation wp_lval := (wp_lval (resolve:=resolve) ti ρ).
+    Local Notation wp_rval := (wp_rval (resolve:=resolve) ti ρ).
+    Local Notation wp_prval := (wp_prval (resolve:=resolve) ti ρ).
+    Local Notation wp_xval := (wp_xval (resolve:=resolve) ti ρ).
+    Local Notation wp_init := (wp_init (resolve:=resolve) ti ρ).
+    Local Notation wpAny := (wpAny (resolve:=resolve) ti ρ).
+    Local Notation wpAnys := (wpAnys (resolve:=resolve) ti ρ).
+    Local Notation fspec := (fspec (resolve:=resolve)).
+
+    Fixpoint is_aggregate (t : type) : bool :=
+      match t with
+      | Tref _
+      | Tarray _ _ => true
+      | Tqualified _ t => is_aggregate t
+      | _ => false
+      end.
+
+    Fixpoint wp_args (es : list (ValCat * Expr)) (Q : list val -> FreeTemps -> mpred) : mpred :=
+      match es with
+      | nil => Q nil empSP
+      | (vc,e) :: es =>
+        let ty := type_of e in
+        match vc with
+        | Lvalue => wp_lval e (fun v free => wp_args es (fun vs frees =>
+                                                       Q (v :: vs) (free ** frees)))
+        | Rvalue =>
+          if is_aggregate ty then
+            Forall a, _at (_eq a) (uninit (erase_qualifiers ty)) -*
+                      wp_init ty a e (fun free => wp_args es (fun vs frees =>
+                                                             Q (a :: vs) (_at (_eq a) (tany (erase_qualifiers ty)) ** free ** frees)))
+          else
+            wp_prval e (fun v free => wp_args es (fun vs frees =>
+                                                Q (v :: vs) (free ** frees)))
+        | Xvalue => wp_xval e (fun v free => wp_args es (fun vs frees =>
+                                                       Q (v :: vs) (free ** frees)))
+        end
+      end.
+    (* todo(gmm): check sequence points *)
+
+  End with_resolve.
+
+End Call.
+
+Declare Module CALL : Call.
+
+Export CALL.
