theories/Sem/Expr.v
@@ -14,7 +14,7 @@ Require Import Coq.Strings.String.
 From Cpp Require Import
      Ast.
 From Cpp.Sem Require Import
-     Util Logic Semantics Operator PLogic Destroy Wp CompilationUnit.
+     ChargeUtil Logic Semantics Operator PLogic Destroy Wp CompilationUnit Call.
 
 Require Import Coq.ZArith.BinInt.
 Require Import Coq.NArith.BinNatDef.
@@ -34,8 +34,13 @@ Module Type Expr.
     Variable ti : thread_info.
     Variable ρ : region.
 
-    Local Notation wp_lhs := (wp_lhs (resolve:=resolve) ti ρ).
-    Local Notation wp_rhs := (wp_rhs (resolve:=resolve) ti ρ).
+    Local Notation wp_lval := (wp_lval (resolve:=resolve) ti ρ).
+    Local Notation wp_prval := (wp_prval (resolve:=resolve) ti ρ).
+    Local Notation wp_xval := (wp_xval (resolve:=resolve) ti ρ).
+    Local Notation wp_glval := (wp_glval (resolve:=resolve) ti ρ).
+    Local Notation wp_rval := (wp_rval (resolve:=resolve) ti ρ).
+    Local Notation wp_init := (wp_init (resolve:=resolve) ti ρ).
+    Local Notation wp_args := (wp_args (resolve:=resolve) ti ρ).
     Local Notation wpAny := (wpAny (resolve:=resolve) ti ρ).
     Local Notation wpe := (wpe (resolve:=resolve) ti ρ).
     Local Notation wpAnys := (wpAnys (resolve:=resolve) ti ρ).
@@ -43,76 +48,136 @@ Module Type Expr.
     Notation "[! P !]" := (embed P).
 
     (* constants are rvalues *)
-    Axiom wp_rhs_constant : forall ty cnst e Q,
-      denoteGlobal cnst (Gconstant ty e) ** wp_rhs e Q
-      |-- wp_rhs (Econst_ref (Gname cnst) ty) Q.
+    Axiom wp_prval_constant : forall ty cnst e Q,
+      denoteGlobal cnst (Gconstant ty e) ** wp_prval e Q
+      |-- wp_prval (Econst_ref (Gname cnst) ty) Q.
 
-    (* integer literals are rvalues *)
-    Axiom wp_rhs_int : forall n ty Q,
+    (* integer literals are prvalues *)
+    Axiom wp_prval_int : forall n ty Q,
       [! has_type (Vint n) (drop_qualifiers ty) !] //\\ Q (Vint n) empSP
-      |-- wp_rhs (Eint n ty) Q.
+      |-- wp_prval (Eint n ty) Q.
 
     (* note that `char` is actually `byte` *)
-    Axiom wp_rhs_char : forall c ty Q,
+    Axiom wp_prval_char : forall c ty Q,
       let n := Ascii.N_of_ascii c in
       [! has_type (Vint n) (drop_qualifiers ty) !] //\\ Q (Vint n) empSP
-      |-- wp_rhs (Echar c ty) Q.
+      |-- wp_prval (Echar c ty) Q.
 
-    (* boolean literals are rvalues *)
-    Axiom wp_rhs_bool : forall (b : bool) Q,
+    (* boolean literals are prvalues *)
+    Axiom wp_prval_bool : forall (b : bool) Q,
       Q (Vint (if b then 1 else 0)) empSP
-      |-- wp_rhs (Ebool b) Q.
+      |-- wp_prval (Ebool b) Q.
 
-    (* `this` is an rvalue *)
-    Axiom wp_rhs_this : forall ty Q,
+    (* `this` is a prvalue *)
+    Axiom wp_prval_this : forall ty Q,
       Exists a, (_this ρ &~ a ** ltrue) //\\ Q a empSP
-      |-- wp_rhs (Ethis ty) Q.
+      |-- wp_prval (Ethis ty) Q.
 
 
     (* variables are lvalues *)
-    Axiom wp_lhs_lvar : forall ty x Q,
+    Axiom wp_lval_lvar : forall ty x Q,
         Exists a, (_local ρ x &~ a ** ltrue) //\\ Q a empSP
-        |-- wp_lhs (Evar (Lname x) ty) Q.
+        |-- wp_lval (Evar (Lname x) ty) Q.
 
     (* what about the type? if it exists *)
-    Axiom wp_lhs_gvar : forall ty x Q,
+    Axiom wp_lval_gvar : forall ty x Q,
         Exists a, [! glob_addr resolve x a !] //\\ Q (Vptr a) empSP
-        |-- wp_lhs (Evar (Gname x) ty) Q.
+        |-- wp_lval (Evar (Gname x) ty) Q.
 
-    (* this is a "prvalue" if
-     * - `e` is a member enumerator or non-static member function
-     * - `e` is an rvalue and `m` is non-static data of non-reference type
+    (* [Emember e f ty] is an lvalue by default except when
+     * - where m is a member enumerator or a non-static member function, or
+     * - where a is an rvalue and m is a non-static data member of non-reference type
      *)
-    Axiom wp_lhs_member : forall ty e f Q,
-      wp_lhs e (fun base free =>
-                  Exists addr, (_offsetL (_field f) (_eq base) &~ addr ** ltrue) //\\ Q addr free)
-      |-- wp_lhs (Emember e f ty) Q.
+    Axiom wp_lval_member : forall ty a m Q,
+      wp_lval a (fun base free =>
+                  Exists addr, (_offsetL (_field m) (_eq base) &~ addr ** ltrue) //\\ Q addr free)
+      |-- wp_lval (Emember a m ty) Q.
 
-    Axiom wp_lhs_subscript : forall e i t Q,
-      wp_rhs e (fun base free =>
-        wp_rhs i (fun idx free' =>
+
+    (* [Emember a m ty] is a prvalue if
+     * - [a] is a member enumerator or non-static member function, or
+     * - [a] is an rvalue and [m] is non-static data of non-reference type
+     *)
+    Axiom wp_prval_member : forall ty a m Q,
+      wp_rval a (fun base free =>
+                  Exists addr, (_offsetL (_field m) (_eq base) &~ addr ** ltrue) //\\ Q addr free)
+      |-- wp_prval (Emember a m ty) Q.
+
+    (* [Emember a m ty] is an xvalue if
+     * - [a] is an rvalue and [m] is a non-static data member of non-reference type
+     *)
+    Axiom wp_xval_member : forall ty a m Q,
+      wp_rval a (fun base free =>
+                  Exists addr, (_offsetL (_field m) (_eq base) &~ addr ** ltrue) //\\ Q addr free)
+      |-- wp_xval (Emember a m ty) Q.
+
+    Fixpoint is_pointer (ty : type) : bool :=
+      match ty with
+      | Tpointer _
+      | Tarray _ _ => true
+      | Tqualified _ t => is_pointer t
+      | _ => false
+      end.
+
+    (* [Esubscript a n ty] is an lvalue if
+     * - one operand is an lvalue array
+     *   (in clang's syntax tree, this value is converted to an rvalue via
+     *    an array2pointer cast)
+     *)
+    Axiom wp_lval_subscript : forall e i t Q,
+      (if is_pointer (type_of e) then
+      wp_prval e (fun base free => (* todo: rval? *)
+        wp_prval i (fun idx free' =>
           Exists addr,
           (Exists i, [| idx = Vint i |] **
-          _offsetL (_sub (drop_qualifiers t) i) (_eq base) &~ addr ** ltrue) //\\
+          _offsetL (_sub (erase_qualifiers t) i) (_eq base) &~ addr ** ltrue) //\\
           Q addr (free' ** free)))
-      |-- wp_lhs (Esubscript e i t) Q.
+      else
+      wp_prval e (fun idx free => (* todo: rval? *)
+        wp_prval i (fun base free' =>
+          Exists addr,
+          (Exists i, [| idx = Vint i |] **
+          _offsetL (_sub (erase_qualifiers t) i) (_eq base) &~ addr ** ltrue) //\\
+          Q addr (free' ** free))))
+      |-- wp_lval (Esubscript e i t) Q.
+
+    (* [Esubscript e i t]
+     * - where one operand is an array rvalue
+     *)
+    Axiom wp_xval_subscript : forall e i t Q,
+      (if is_pointer (type_of e) then
+      wp_prval e (fun base free => (* todo: rval? *)
+        wp_prval i (fun idx free' =>
+          Exists addr,
+          (Exists i, [| idx = Vint i |] **
+          _offsetL (_sub (erase_qualifiers t) i) (_eq base) &~ addr ** ltrue) //\\
+          Q addr (free' ** free)))
+      else
+      wp_prval e (fun idx free => (* todo: rval? *)
+        wp_prval i (fun base free' =>
+          Exists addr,
+          (Exists i, [| idx = Vint i |] **
+          _offsetL (_sub (erase_qualifiers t) i) (_eq base) &~ addr ** ltrue) //\\
+          Q addr (free' ** free))))
+      |-- wp_xval (Esubscript e i t) Q.
+
 
     (* the `*` operator is an lvalue *)
-    Axiom wp_lhs_deref : forall ty e Q,
-        wp_rhs e Q
-        |-- wp_lhs (Ederef e ty) Q.
+    Axiom wp_lval_deref : forall ty e Q,
+        wp_prval e Q (* todo: rval? *)
+        |-- wp_lval (Ederef e ty) Q.
 
     (* the `&` operator is a prvalue *)
-    Axiom wp_rhs_addrof : forall ty e Q,
-        wp_lhs e Q
-        |-- wp_rhs (Eaddrof e ty) Q.
+    Axiom wp_prval_addrof : forall ty e Q,
+        wp_lval e Q
+        |-- wp_prval (Eaddrof e ty) Q.
 
     (* unary operators *)
-    Axiom wp_rhs_unop : forall o e ty Q,
-        wp_rhs e (fun v free =>
+    Axiom wp_prval_unop : forall o e ty Q,
+        wp_prval e (fun v free => (* todo: rval? *)
           Exists v',
-          embed (eval_unop (resolve:=resolve) o (drop_qualifiers (type_of e)) (drop_qualifiers ty) v v') //\\ Q v' free)
-        |-- wp_rhs (Eunop o e ty) Q.
+          embed (eval_unop (resolve:=resolve) o (erase_qualifiers (type_of e)) (erase_qualifiers ty) v v') //\\ Q v' free)
+        |-- wp_prval (Eunop o e ty) Q.
 
     (* note(gmm): operators need types! *)
     Fixpoint companion_type (t : type) : option type :=
@@ -124,65 +189,65 @@ Module Type Expr.
       | _ => None
       end.
 
-    Axiom wp_lhs_preinc : forall e ty Q,
+    Axiom wp_lval_preinc : forall e ty Q,
         match companion_type (type_of e) with
         | Some cty =>
-          wp_lhs e (fun a free => Exists v', Exists v'',
-              _at (_eq a) (tprim (drop_qualifiers ty) v') **
-              [| eval_binop (resolve:=resolve) Badd (drop_qualifiers (type_of e)) cty (drop_qualifiers ty) v' (Vint 1) v'' |] **
-              (_at (_eq a) (tprim (drop_qualifiers ty) v'') -* Q a free))
+          wp_lval e (fun a free => Exists v', Exists v'',
+              _at (_eq a) (tprim (erase_qualifiers ty) v') **
+              [| eval_binop (resolve:=resolve) Badd (erase_qualifiers (type_of e)) cty (erase_qualifiers ty) v' (Vint 1) v'' |] **
+              (_at (_eq a) (tprim (erase_qualifiers ty) v'') -* Q a free))
         | None => lfalse
         end
-        |-- wp_lhs (Epreinc e ty) Q.
+        |-- wp_lval (Epreinc e ty) Q.
 
-    Axiom wp_lhs_predec : forall e ty Q,
+    Axiom wp_lval_predec : forall e ty Q,
         match companion_type (type_of e) with
         | Some cty =>
-          wp_lhs e (fun a free => Exists v', Exists v'',
-              _at (_eq a) (tprim (drop_qualifiers ty) v') **
-              [| eval_binop (resolve:=resolve) Bsub (drop_qualifiers (type_of e)) cty (drop_qualifiers ty) v' (Vint 1) v'' |] **
-              (_at (_eq a) (tprim (drop_qualifiers ty) v'') -* Q a free))
+          wp_lval e (fun a free => Exists v', Exists v'',
+              _at (_eq a) (tprim (erase_qualifiers ty) v') **
+              [| eval_binop (resolve:=resolve) Bsub (erase_qualifiers (type_of e)) cty (erase_qualifiers ty) v' (Vint 1) v'' |] **
+              (_at (_eq a) (tprim (erase_qualifiers ty) v'') -* Q a free))
         | None => lfalse
         end
-        |-- wp_lhs (Epredec e ty) Q.
+        |-- wp_lval (Epredec e ty) Q.
 
-    Axiom wp_rhs_postinc : forall e ty Q,
+    Axiom wp_prval_postinc : forall e ty Q,
         match companion_type (type_of e) with
         | Some cty =>
-          wp_lhs e (fun a free => Exists v', Exists v'',
-              _at (_eq a) (tprim (drop_qualifiers ty) v') **
-              [| eval_binop (resolve:=resolve) Badd (drop_qualifiers (type_of e)) cty (drop_qualifiers ty) v' (Vint 1) v'' |] **
-              (_at (_eq a) (tprim (drop_qualifiers ty) v'') -* Q v' free))
+          wp_lval e (fun a free => Exists v', Exists v'',
+              _at (_eq a) (tprim (erase_qualifiers ty) v') **
+              [| eval_binop (resolve:=resolve) Badd (erase_qualifiers (type_of e)) cty (erase_qualifiers ty) v' (Vint 1) v'' |] **
+              (_at (_eq a) (tprim (erase_qualifiers ty) v'') -* Q v' free))
         | None => lfalse
         end
-        |-- wp_rhs (Epostinc e ty) Q.
+        |-- wp_prval (Epostinc e ty) Q.
 
-    Axiom wp_rhs_postdec : forall e ty Q,
+    Axiom wp_prval_postdec : forall e ty Q,
         match companion_type (type_of e) with
         | Some cty =>
-          wp_lhs e (fun a free => Exists v', Exists v'',
-              _at (_eq a) (tprim (drop_qualifiers ty) v') **
-              [| eval_binop (resolve:=resolve) Bsub (drop_qualifiers (type_of e)) cty (drop_qualifiers ty) v' (Vint 1) v'' |] **
-              (_at (_eq a) (tprim (drop_qualifiers ty) v'') -* Q v' free))
+          wp_lval e (fun a free => Exists v', Exists v'',
+              _at (_eq a) (tprim (erase_qualifiers ty) v') **
+              [| eval_binop (resolve:=resolve) Bsub (erase_qualifiers (type_of e)) cty (erase_qualifiers ty) v' (Vint 1) v'' |] **
+              (_at (_eq a) (tprim (erase_qualifiers ty) v'') -* Q v' free))
         | None => lfalse
         end
-        |-- wp_rhs (Epostdec e ty) Q.
+        |-- wp_prval (Epostdec e ty) Q.
 
     (** binary operators *)
-    Axiom wp_rhs_binop : forall o e1 e2 ty Q,
-        wp_rhs e1 (fun v1 free1 => wp_rhs e2 (fun v2 free2 =>
-            Exists v', embed (eval_binop (resolve:=resolve) o (drop_qualifiers (type_of e1)) (drop_qualifiers (type_of e2)) (drop_qualifiers ty) v1 v2 v') //\\ Q v' (free1 ** free2)))
-        |-- wp_rhs (Ebinop o e1 e2 ty) Q.
+    Axiom wp_prval_binop : forall o e1 e2 ty Q,
+        wp_prval e1 (fun v1 free1 => wp_prval e2 (fun v2 free2 =>
+            Exists v', embed (eval_binop (resolve:=resolve) o (erase_qualifiers (type_of e1)) (erase_qualifiers (type_of e2)) (erase_qualifiers ty) v1 v2 v') //\\ Q v' (free1 ** free2)))
+        |-- wp_prval (Ebinop o e1 e2 ty) Q.
 
-    Axiom wp_lhs_assign : forall ty l r Q,
-        wp_lhs l (fun la free1 => wp_rhs r (fun rv free2 =>
-            _at (_eq la) (tany (drop_qualifiers ty)) **
-           (_at (_eq la) (tprim (drop_qualifiers ty) rv) -* Q la (free1 ** free2))))
-        |-- wp_lhs (Eassign l r ty) Q.
+    Axiom wp_lval_assign : forall ty l r Q,
+        wp_lval l (fun la free1 => wp_prval r (fun rv free2 =>
+            _at (_eq la) (tany (erase_qualifiers ty)) **
+           (_at (_eq la) (tprim (erase_qualifiers ty) rv) -* Q la (free1 ** free2))))
+        |-- wp_lval (Eassign l r ty) Q.
 
-    Axiom wp_lhs_bop_assign : forall ty o l r Q,
-        wp_lhs (Eassign l (Ebinop o (Ecast Cl2r (Lvalue, l) (type_of l)) r ty) ty) Q
-        |-- wp_lhs (Eassign_op o l r ty) Q.
+    Axiom wp_lval_bop_assign : forall ty o l r Q,
+        wp_lval (Eassign l (Ebinop o (Ecast Cl2r (Lvalue, l) (type_of l)) r ty) ty) Q
+        |-- wp_lval (Eassign_op o l r ty) Q.
 
     (* note: the comma operator can be both an lvalue and a prvalue
      * depending on what the second expression is.
@@ -193,160 +258,240 @@ Module Type Expr.
         |-- wpe m (Ecomma vc e1 e2 ty) Q.
 
     (** short-circuting operators *)
-    Axiom wp_rhs_seqand : forall ty e1 e2 Q,
-        wp_rhs e1 (fun v1 free1 =>
+    Axiom wp_prval_seqand : forall ty e1 e2 Q,
+        wp_prval e1 (fun v1 free1 => (* todo: rval? *)
            if is_true v1
-           then wp_rhs e2 (fun v2 free2 =>
+           then wp_prval e2 (fun v2 free2 => (* todo: rval? *)
                                      if is_true v2
                                      then Q (Vint 1) (free1 ** free2)
                                      else Q (Vint 0) (free1 ** free2))
            else Q (Vint 0) free1)
-        |-- wp_rhs (Eseqand e1 e2 ty) Q.
+        |-- wp_prval (Eseqand e1 e2 ty) Q.
 
-    Axiom wp_rhs_seqor : forall ty e1 e2 Q,
-        wp_rhs e1 (fun v1 free1 =>
+    Axiom wp_prval_seqor : forall ty e1 e2 Q,
+        wp_prval e1 (fun v1 free1 => (* todo: rval? *)
            if is_true v1
            then Q (Vint 1) free1
-           else wp_rhs e2 (fun v2 free2 =>
+           else wp_prval e2 (fun v2 free2 => (* todo: rval? *)
                                      if is_true v2
                                      then Q (Vint 1) (free1 ** free2)
                                      else Q (Vint 0) (free1 ** free2)))
-        |-- wp_rhs (Eseqor e1 e2 ty) Q.
+        |-- wp_prval (Eseqor e1 e2 ty) Q.
 
     (** casts *)
-    Axiom wp_rhs_cast_l2r : forall ty e Q,
-        wp_lhs e (fun a free =>
-          Exists v, (_at (_eq a) (tprim (drop_qualifiers ty) v) ** ltrue) //\\
+    Axiom wp_prval_cast_l2r_l : forall ty e Q,
+        wp_lval e (fun a free => (* was wp_lval *)
+          Exists v, (_at (_eq a) (tprim (erase_qualifiers ty) v) ** ltrue) //\\
                     Q v free)
-        |-- wp_rhs (Ecast Cl2r (Lvalue, e) ty) Q.
+        |-- wp_prval (Ecast Cl2r (Lvalue, e) ty) Q.
 
-    Axiom wpe_cast_noop : forall ty m e Q,
-        wpe m e Q
-        |-- wpe m (Ecast Cnoop (m, e) ty) Q.
+    Axiom wp_prval_cast_l2r_x : forall ty e Q,
+        wp_xval e (fun a free => (* was wp_lval *)
+          Exists v, (_at (_eq a) (tprim (erase_qualifiers ty) v) ** ltrue) //\\
+                    Q v free)
+        |-- wp_prval (Ecast Cl2r (Xvalue, e) ty) Q.
 
-    Axiom wp_rhs_cast_int2bool : forall ty e Q,
-        wp_rhs e Q
-        |-- wp_rhs (Ecast Cint2bool (Rvalue, e) ty) Q.
+    Axiom wp_prval_cast_noop : forall ty e Q,
+        wp_prval e Q
+        |-- wp_prval (Ecast Cnoop (Rvalue, e) ty) Q.
+    Axiom wp_lval_cast_noop : forall ty e Q,
+        wp_lval e Q
+        |-- wp_lval (Ecast Cnoop (Lvalue, e) ty) Q.
+    Axiom wp_xval_cast_noop : forall ty e Q,
+        wp_xval e Q
+        |-- wp_xval (Ecast Cnoop (Xvalue, e) ty) Q.
+    Axiom wp_lval_xval_cast_noop : forall ty e Q,
+        wp_xval e Q
+        |-- wp_lval (Ecast Cnoop (Xvalue, e) ty) Q.
+    Axiom wp_xval_lval_cast_noop : forall ty e Q,
+        wp_lval e Q
+        |-- wp_xval (Ecast Cnoop (Lvalue, e) ty) Q.
+
+    Axiom wp_prval_cast_int2bool : forall ty e Q,
+        wp_prval e Q
+        |-- wp_prval (Ecast Cint2bool (Rvalue, e) ty) Q.
     (* ^ todo(gmm): confirm that this doesn't change the value *)
 
-    Axiom wp_rhs_cast_ptr2bool : forall ty e Q,
-        wp_rhs e Q
-        |-- wp_rhs (Ecast Cptr2bool (Rvalue, e) ty) Q.
+    Axiom wp_prval_cast_ptr2bool : forall ty e Q,
+        wp_prval e Q
+        |-- wp_prval (Ecast Cptr2bool (Rvalue, e) ty) Q.
     (* ^ todo(gmm): confirm that this doesn't change the value *)
 
-    Axiom wp_rhs_cast_function2pointer_c : forall ty ty' g Q,
-        wp_lhs (Evar (Gname g) ty') Q
-        |-- wp_rhs (Ecast Cfunction2pointer (Rvalue, Evar (Gname g) ty') ty) Q.
-    Axiom wp_rhs_cast_function2pointer_cpp : forall ty ty' g Q,
-        wp_lhs (Evar (Gname g) ty') Q
-        |-- wp_rhs (Ecast Cfunction2pointer (Lvalue, Evar (Gname g) ty') ty) Q.
+    Axiom wp_prval_cast_function2pointer_c : forall ty ty' g Q,
+        wp_lval (Evar (Gname g) ty') Q
+        |-- wp_prval (Ecast Cfunction2pointer (Rvalue, Evar (Gname g) ty') ty) Q.
+    Axiom wp_prval_cast_function2pointer_cpp : forall ty ty' g Q,
+        wp_lval (Evar (Gname g) ty') Q
+        |-- wp_prval (Ecast Cfunction2pointer (Lvalue, Evar (Gname g) ty') ty) Q.
     (* ^ note(gmm): C and C++ classify function names differently
      * - in C, function names are Rvalues, and
      * - in C++, function names are Lvalues
      *)
 
-    Axiom wp_rhs_cast_bitcast : forall e t Q,
-        wp_rhs e Q
-        |-- wp_rhs (Ecast Cbitcast (Rvalue, e) t) Q.
+    Axiom wp_prval_cast_bitcast : forall e t Q,
+        wp_prval e Q
+        |-- wp_prval (Ecast Cbitcast (Rvalue, e) t) Q.
 
-    Axiom wp_rhs_cast_integral : forall e t Q,
-        wp_rhs e (fun v free => [| has_type v t |] ** Q v free)
-        |-- wp_rhs (Ecast Cintegral (Rvalue, e) t) Q.
+    Axiom wp_prval_cast_integral : forall e t Q,
+        wp_prval e (fun v free => [| has_type v t |] ** Q v free)
+        |-- wp_prval (Ecast Cintegral (Rvalue, e) t) Q.
 
-    Axiom wp_rhs_cast_null : forall e t Q,
-        wp_rhs e Q
-        |-- wp_rhs (Ecast Cnull2ptr (Rvalue, e) t) Q.
+    Axiom wp_prval_cast_null : forall e t Q,
+        wp_prval e Q
+        |-- wp_prval (Ecast Cnull2ptr (Rvalue, e) t) Q.
     (* ^ todo(jmgrosen): confirm that this doesn't change the value *)
 
     (* note(gmm): in the clang AST, the subexpression is the call.
      * in essence, `Ecast (Cuser ..)` is a syntax annotation.
      *)
-    Axiom wp_rhs_cast_user : forall e ty Z Q,
-        wp_rhs e Q
-        |-- wp_rhs (Ecast (Cuser Z) (Rvalue, e) ty) Q.
+    Axiom wp_prval_cast_user : forall e ty Z Q,
+        wp_prval e Q
+        |-- wp_prval (Ecast (Cuser Z) (Rvalue, e) ty) Q.
 
-    Axiom wp_rhs_cast_reinterpret : forall q e ty Q,
-        wp_rhs e Q |-- wp_rhs (Ecast (Creinterpret q) (Rvalue, e) ty) Q.
+    Axiom wp_prval_cast_reinterpret : forall q e ty Q,
+        wp_prval e Q
+        |-- wp_prval (Ecast (Creinterpret q) (Rvalue, e) ty) Q.
 
-    Axiom wp_lhs_static_cast : forall vc from to e ty Q,
+    Axiom wp_lval_static_cast : forall vc from to e ty Q,
       wpe vc e (fun addr free => Exists addr',
                   (_offsetL (_super from to) (_eq addr) &~ addr' //\\ ltrue) **
                           (* ^ this is a down-cast *)
                   Q addr' free)
-      |-- wp_lhs (Ecast (Cstatic from to) (vc, e) ty) Q.
+      |-- wp_lval (Ecast (Cstatic from to) (vc, e) ty) Q.
 
-    Axiom wpe_cast_tovoid : forall vc e ty Q,
+    Axiom wpe_cast_tovoid : forall vc' vc e ty Q,
       wpe vc e (fun _ free => Q (Vint 0) free)
-      |-- wpe vc (Ecast C2void (vc, e) ty) Q.
+      |-- wpe vc' (Ecast C2void (vc, e) ty) Q.
 
-    Axiom wp_rhs_cast_array2pointer : forall e t Q,
-        wp_lhs e Q
-        |-- wp_rhs (Ecast Carray2pointer (Lvalue, e) t) Q.
+    Axiom wp_prval_cast_array2pointer : forall e t Q,
+        wp_lval e Q
+        |-- wp_prval (Ecast Carray2pointer (Lvalue, e) t) Q.
 
     (** the ternary operator `_ ? _ : _` *)
     Axiom wp_condition : forall ty m tst th el Q,
-        wp_rhs tst (fun v1 free =>
+        wp_prval tst (fun v1 free => (* todo: rval? *)
            if is_true v1
-           then wpe m th (fun v free' => Q v (free ** free'))
-           else wpe m el (fun v free' => Q v (free ** free')))
+           then wpe m th (fun v free' => free ** Q v free')
+           else wpe m el (fun v free' => free ** Q v free'))
         |-- wpe m (Eif tst th el ty) Q.
-    (* ^ todo(gmm): it would be sound for `free` to occur in the branches *)
 
     (** `sizeof` and `alignof` *)
-    Axiom wp_rhs_sizeof : forall ty' ty Q,
+    Axiom wp_prval_sizeof : forall ty' ty Q,
         Exists sz, [| @size_of resolve ty sz |] ** Q (Vint (Z.of_N sz)) empSP
-        |-- wp_rhs (Esize_of (inl ty) ty') Q.
+        |-- wp_prval (Esize_of (inl ty) ty') Q.
 
-    Axiom wp_rhs_sizeof_e : forall ty' e Q,
-        wp_rhs (Esize_of (inl (type_of e)) ty') Q
-        |-- wp_rhs (Esize_of (inr e) ty') Q.
+    Axiom wp_prval_sizeof_e : forall ty' e Q,
+        wp_prval (Esize_of (inl (type_of e)) ty') Q
+        |-- wp_prval (Esize_of (inr e) ty') Q.
 
-
-    Axiom wp_rhs_alignof : forall ty' ty Q,
+    Axiom wp_prval_alignof : forall ty' ty Q,
         Exists sz, [| @align_of resolve ty sz |] ** Q (Vint (Z.of_N sz)) empSP
-        |-- wp_rhs (Ealign_of (inl ty) ty') Q.
+        |-- wp_prval (Ealign_of (inl ty) ty') Q.
 
-    Axiom wp_rhs_alignof_e : forall ty' e Q,
-        wp_rhs (Ealign_of (inl (type_of e)) ty') Q
-        |-- wp_rhs (Ealign_of (inr e) ty') Q.
-
-    (** constructors *)
-    Axiom wp_rhs_constructor
-    : forall cls cname (es : list (ValCat * Expr)) (ty : type) (Q : val -> FreeTemps -> mpred),
-     (Exists ctor, [| glob_addr resolve cname ctor |] **
-      wps wpAnys es (fun vs free => Exists a, _at (_eq a) (uninit (Tref cls))
-          -* |> fspec (resolve:=resolve) (Vptr ctor) (a :: vs) ti (fun _ =>
-                   (* note(gmm): constructors are rvalues but my semantics actually
-                    * treats them like lvalues. *)
-                   Q a (destroy (resolve:=resolve) ti Dt_Complete cls a free))) empSP)
-      |-- wp_rhs (Econstructor cname es (Tref cls)) Q.
+    Axiom wp_prval_alignof_e : forall ty' e Q,
+        wp_prval (Ealign_of (inl (type_of e)) ty') Q
+        |-- wp_prval (Ealign_of (inr e) ty') Q.
 
     (** function calls *)
-    Axiom wp_call : forall ty f es Q,
-        wp_rhs f (fun f => wps wpAnys es (fun vs free =>
-            |> fspec (resolve:=resolve) f vs ti (fun v => Q v free)))
-        |-- wp_rhs (Ecall f es ty) Q.
+    Axiom wp_prval_call : forall ty f es Q,
+        (if is_aggregate ty then
+          Forall addr, wp_init ty addr (Ecall f es ty) (fun free =>
+            Q addr (free ** _at (_eq addr) (tany (erase_qualifiers ty))))
+        else
+          wp_prval f (fun f free => wp_args es (fun vs free' =>
+            |> fspec (resolve:=resolve) f vs ti (fun v => Q v (free ** free')))))
+        |-- wp_prval (Ecall f es ty) Q.
+    Axiom wp_xval_call : forall ty f es Q,
+        wp_prval f (fun f free => wp_args es (fun vs free' =>
+            |> fspec (resolve:=resolve) f vs ti (fun v => Q v (free ** free'))))
+        |-- wp_xval (Ecall f es ty) Q.
+    Axiom wp_init_call :
+      forall f (es : list (ValCat * Expr))
+        (Q : FreeTemps -> mpred) addr (ty : type),
+        wp_prval f (fun f free_f => wp_args es (fun vs free_args =>
+             |> fspec (resolve:=resolve) f vs ti (fun res =>
+                      [| res = addr |] -* Q (free_f ** free_args))))
+        |-- wp_init ty addr (Ecall f es ty) Q.
 
-    Axiom wp_member_call : forall ty f obj es Q,
+    Axiom wp_prval_member_call : forall ty f obj es Q,
         Exists fa, [| glob_addr resolve f fa |] **
-        wp_lhs obj (fun this => wps wpAnys es (fun vs free =>
-            |> fspec (resolve:=resolve) (Vptr fa) (this :: vs) ti (fun v => Q v free)))
-        |-- wp_rhs (Emember_call false f obj es ty) Q.
+        wp_lval obj (fun this free => wp_args es (fun vs free' =>
+            |> fspec (resolve:=resolve) (Vptr fa) (this :: vs) ti (fun v => Q v (free ** free'))))
+        |-- wp_prval (Emember_call false f obj es ty) Q.
+    Axiom wp_xval_member_call : forall ty f obj es Q,
+        Exists fa, [| glob_addr resolve f fa |] **
+        wp_lval obj (fun this free => wp_args es (fun vs free' =>
+            |> fspec (resolve:=resolve) (Vptr fa) (this :: vs) ti (fun v => Q v (free ** free'))))
+        |-- wp_xval (Emember_call false f obj es ty) Q.
+    Axiom wp_init_member_call :
+      forall f (es : list (ValCat * Expr))
+        (Q : FreeTemps -> mpred) addr (ty : type) obj,
+        Exists fa, [| glob_addr resolve f fa |] **
+        wp_prval obj (fun this free_o => wp_args es (fun vs free_args =>
+             |> fspec (resolve:=resolve) (Vptr fa) (this :: vs) ti (fun res =>
+                      [| res = addr |] -* Q (free_o ** free_args))))
+        |-- wp_init ty addr (Emember_call false f obj es ty) Q.
 
     (* null *)
     Axiom wp_null : forall Q,
         Q (Vptr nullptr) empSP
-        |-- wp_rhs Enull Q.
+        |-- wp_prval Enull Q.
 
     (* temporary expressions
      * note(gmm): these axioms should be reviewed thoroughly
      *)
-    Axiom wp_rhs_clean : forall e ty Q,
-        wp_rhs e Q
-        |-- wp_rhs (Eandclean e ty) Q.
-    Axiom wp_lhs_temp : forall e ty Q,
-        wp_rhs e Q
-        |-- wp_lhs (Ematerialize_temp e ty) Q.
+    Axiom wp_lval_clean : forall e ty Q,
+        wp_lval e Q |-- wp_lval (Eandclean e ty) Q.
+    Axiom wp_prval_clean : forall e ty Q,
+        wp_prval e Q |-- wp_prval (Eandclean e ty) Q.
+    Axiom wp_xval_clean : forall e ty Q,
+        wp_xval e Q |-- wp_xval (Eandclean e ty) Q.
+
+    (* [Ematerialize_temp e ty] is an xvalue
+     *)
+    Axiom wp_xval_temp : forall e ty Q,
+        Forall a, _at (_eq a) (uninit (erase_qualifiers ty)) -*
+                  wp_init ty a e
+                          (fun free => free ** Q a (_at (_eq a) (tany (erase_qualifiers ty))))
+        |-- wp_xval (Ematerialize_temp e ty) Q.
+
+    (* [Ematerialize_temp e ty] is an xvalue
+     *)
+    Axiom wp_lval_temp : forall e ty Q,
+        Forall a, _at (_eq a) (uninit (erase_qualifiers ty)) -*
+                  wp_init ty a e
+                          (fun free => free ** Q a (_at (_eq a) (tany (erase_qualifiers ty))))
+        |-- wp_lval (Ematerialize_temp e ty) Q.
+
+    (* temporary materialization only occurs when the resulting value is used.
+     * if the value is ignored, e.g. in `go();` (when the result of `go` is an
+     * aggregate) we introduce an implicit materialization and then immediately
+     * free the result.
+     *)
+    Axiom wp_prval_implicit_materialize : forall e Q,
+        is_aggregate (type_of e) = true ->
+        (Forall a, _at (_eq a) (uninit (erase_qualifiers (type_of e))) -*
+                   wp_init (type_of e) a e (fun free =>
+                                              Q a (_at (_eq a) (tany (type_of e)) ** free)))
+        |-- wp_prval e Q.
+
+
+    (* [Ebind_temp e dtor ty] is an initialization expression that ensures
+     * that the destructor is called.
+     *)
+    Axiom wp_init_bind_temp : forall e ty a dtor Q,
+        wp_init ty a e (fun free =>
+                     Exists fa, [| glob_addr resolve dtor fa |] **
+                     |> fspec (resolve:=resolve) (Vptr fa) (a :: nil) ti (fun _ => Q free))
+        |-- wp_init ty a (Ebind_temp e dtor ty) Q.
+
+
+    Axiom wp_prval_materialize : forall ty e dtor Q,
+      Forall a : val,
+      _at (_eq a) (uninit (erase_qualifiers ty)) -*
+          wp_init ty a (Ebind_temp e dtor ty)
+          (fun free : FreeTemps => Q a (_at (_eq a) (tany (erase_qualifiers ty)) ** free))
+       |-- wp_prval (Ebind_temp e dtor ty) Q.
 
 
   End with_resolve.
