theories/Sem/Init.v
@@ -3,15 +3,17 @@
  *
  * SPDX-License-Identifier:AGPL-3.0-or-later
  *)
+Require Import Coq.ZArith.ZArith.
 Require Import Coq.Lists.List.
 Require Import Coq.Strings.String.
 
 Local Open Scope string_scope.
+Local Open Scope Z_scope.
 
 From Cpp Require Import
      Ast.
 From Cpp.Sem Require Import
-     Util Logic PLogic Semantics Wp.
+     ChargeUtil Logic PLogic Semantics Call Wp.
 
 Module Type Init.
 
@@ -22,8 +24,12 @@ Module Type Init.
 
     Local Notation wp := (wp (resolve:=resolve)  ti ρ).
     Local Notation wpe := (wpe (resolve:=resolve) ti ρ).
-    Local Notation wp_lhs := (wp_lhs (resolve:=resolve) ti ρ).
-    Local Notation wp_rhs := (wp_rhs (resolve:=resolve) ti ρ).
+    Local Notation wp_lval := (wp_lval (resolve:=resolve) ti ρ).
+    Local Notation wp_rval := (wp_rval (resolve:=resolve) ti ρ).
+    Local Notation wp_prval := (wp_prval (resolve:=resolve) ti ρ).
+    Local Notation wp_xval := (wp_xval (resolve:=resolve) ti ρ).
+    Local Notation wp_init := (wp_init (resolve:=resolve) ti ρ).
+    Local Notation wp_args := (wp_args (resolve:=resolve) ti ρ).
     Local Notation wpAny := (wpAny (resolve:=resolve) ti ρ).
     Local Notation wpAnys := (wpAnys (resolve:=resolve) ti ρ).
     Local Notation fspec := (fspec (resolve:=resolve)).
@@ -31,63 +37,103 @@ Module Type Init.
     (** initialization lists *)
     Parameter wpi
     : forall {resolve : genv} (ti : thread_info) (ρ : region)
-        (cls : globname) (this : val) (init : FieldOrBase * Expr)
-        (Q : mpred), mpred.
+        (cls : globname) (this : val) (init : Initializer)
+        (Q : mpred -> mpred), mpred.
 
-    Fixpoint wpis (cls : globname) (this : val)
-             (inits : list (FieldOrBase * Expr))
-             (Q : mpred) : mpred :=
-      match inits with
-      | nil => Q
-      | i :: is => @wpi resolve ti ρ cls this i (wpis cls this is Q)
-      end.
-
-    Fixpoint wpi_init (cls : globname) (this : Loc)
-             (ty : type) (off : Offset) (init : Expr)
-             (k : mpred)
-    : mpred :=
+    (* this is really about expression evaluation, so it doesn't make sense for
+     * it to be recursive on a type.
+     *)
+    Fixpoint wp_initialize (ty : type) (addr : val) (init : Expr) (k : FreeTemps -> mpred)
+    {struct ty} : mpred :=
       match ty with
-      | Trv_reference t
-      | Treference t =>
-        (* i should use the type here *)
-        wp_lhs init (fun a free =>
-              (* note(gmm): this is consistent with the specification,
-               * but also very strange *)
-              _offsetL off this &~ a
-           -* (free ** k))
-      | Tfunction _ _ =>
-        (* fields can not be function type *)
-        lfalse
       | Tvoid => lfalse
       | Tpointer _
       | Tbool
       | Tchar _ _
       | Tint _ _ =>
-        wp_rhs init (fun v free =>
-           _at (_offsetL off this) (uninit ty) **
-           (   _at (_offsetL off this) (tprim ty v)
-            -* (free ** k)))
-      | Tarray _ _ => lfalse (* todo(gmm): arrays not yet supported *)
-      | Tref gn =>
-        match init with
-        | Econstructor cnd es _ =>
-          (* todo(gmm): constructors need to be handled through `cglob`.
-           *)
-          Exists ctor, [| glob_addr resolve cnd ctor |] **
-          (* todo(gmm): is there a better way to get the destructor? *)
-          wps wpAnys es (fun vs free =>
-              Forall a, (_offsetL off this &~ a ** ltrue) //\\
-              |> fspec (Vptr ctor) (a :: vs) ti (fun _ =>
-                 (free ** k))) empSP
-        | _ => lfalse
-          (* ^ all non-primitive declarations must have initializers *)
-        end
-      | Tqualified _ ty => wpi_init cls this ty off init k
+        wp_prval init (fun v free =>
+                         _at (_eq addr) (uninit (erase_qualifiers ty)) **
+                         (   _at (_eq addr) (tprim (erase_qualifiers ty) v)
+                          -* k free))
+
+        (* non-primitives are handled via prvalue-initialization semantics *)
+      | Tarray ety sz => wp_init ty addr init k
+      | Tref gn => wp_init ty addr init k
+      | Treference t => lfalse (* reference fields are not supported *)
+      | Trv_reference t => lfalse (* reference fields are not supported *)
+      | Tfunction _ _ => lfalse (* functions not supported *)
+
+      | Tqualified _ ty => wp_initialize ty addr init k
       end.
 
-    Axiom wpi_initialize : forall this_val e cls path Q,
-        wpi_init cls (_eq this_val) (drop_qualifiers (type_of e)) (offset_for cls path) e Q
-        |-- @wpi resolve ti ρ cls this_val (path, e) Q.
+    Axiom wpi_initialize : forall this_val i cls Q,
+        Exists a,
+          _offsetL (offset_for cls i.(init_path)) (_eq this_val) &~ a ** ltrue //\\
+        wp_initialize (erase_qualifiers i.(init_type)) a i.(init_init) Q
+        |-- @wpi resolve ti ρ cls this_val i Q.
+
+    Fixpoint wpis (cls : globname) (this : val)
+             (inits : list Initializer)
+             (Q : mpred -> mpred) : mpred :=
+      match inits with
+      | nil => Q empSP
+      | i :: is => @wpi resolve ti ρ cls this i (fun f => f ** wpis cls this is Q)
+      end.
+
+    Axiom wp_init_constructor : forall cls addr cnd es Q ty,
+      wp_args es (fun ls free =>
+         Exists ctor, [| glob_addr resolve cnd ctor |] **
+         |> fspec (Vptr ctor) (addr :: ls) ti (fun _ => Q free))
+      |-- wp_init (Tref cls) addr (Econstructor cnd es ty) Q.
+
+    Definition build_array (es : list Expr) (fill : option Expr) (sz : nat)
+    : option (list (Z * Expr)) :=
+      if Nat.ltb (List.length es) sz then
+        match fill with
+        | None => None
+        | Some f =>
+          Some (List.combine (List.map Z.of_nat (seq 0 sz))
+                             (List.app es (map (fun _ => f) (seq (List.length es) (sz - 1)))))
+        end
+      else
+        Some (List.combine (List.map Z.of_nat (seq 0 sz))
+                           (firstn sz es)).
+
+    Axiom wp_init_initlist_array :forall ls fill ety sz addr Q,
+      match build_array ls fill (N.to_nat sz) with
+      | None => lfalse
+      | Some array_list =>
+        _at (_eq addr) (uninit (erase_qualifiers (Tarray ety sz))) **
+          wps (fun '(i,e) (Q : unit -> mpred -> mpred) f =>
+                 Forall a, _offsetL (_sub ety i) (_eq addr) &~ a -*
+                 wp_init ety a e (fun f' => Q tt (f ** f')))
+              array_list
+              (fun _ free => Q free) empSP
+      end
+      |-- wp_init (Tarray ety sz) addr (Einitlist ls fill (Tarray ety sz)) Q.
+
+(*
+
+    Axiom wp_init_wp_init' : forall addr ty init k,
+        wp_init' addr ty init k -|- wp_init addr ty init k.
+*)
+
+    Axiom wp_init_bind_temp : forall e ty dtor loc ty' Q,
+        wp_init loc ty e Q
+        |-- wp_init loc ty (Ebind_temp e dtor ty') Q.
+    Axiom wp_init_cast_noop : forall e ty loc ty' Q,
+        wp_init loc ty e Q
+        |-- wp_init loc ty (Ecast Cnoop (Rvalue, e) ty') Q.
+
+    Axiom wp_init_clean : forall e ty ty' addr Q,
+        wp_init ty' addr e Q
+        |-- wp_init ty' addr (Eandclean e ty) Q.
+    Axiom wp_init_const : forall ty addr e Q,
+        wp_init ty addr e Q
+        |-- wp_init (Qconst ty) addr e Q.
+    Axiom wp_init_mut : forall ty addr e Q,
+        wp_init ty addr e Q
+        |-- wp_init (Qmut ty) addr e Q.
 
   End with_resolve.
 
