tests/rules.mk
@@ -3,43 +3,12 @@
 #
 # SPDX-License-Identifier:AGPL-3.0-or-later
 #
-CS=$(wildcard *.c)
-HS=$(wildcard *.h)
-CPPS=$(wildcard *.cpp)
-HPPS=$(wildcard *.hpp)
-CPP2V?=$(shell dirname $(abspath $(lastword $(MAKEFILE_LIST))))/../build/cpp2v
-
-VS=$(patsubst %.h,%_h.v,$(HS)) $(patsubst %.hpp,%_hpp.v,$(HPPS)) $(patsubst %.c,%_c.v,$(CS)) $(patsubst %.cpp,%_cpp.v,$(CPPS))
-VOS=$(patsubst %.v,%.vo,$(VS))
-
-CFLAGS=
-
-coq: Makefile.coq $(VS)
+coq: Makefile.coq
 	$(MAKE) -f Makefile.coq
 
 clean:
-	@ rm $(VS) -rf $(VOS)
-
-%_c.v: %.c $(CPP2V)
-	$(CPP2V) -o $@ $< -- $(CFLAGS)
-%_h.v: %.h $(CPP2V)
-	$(CPP2V) -o $@ $< -- $(CFLAGS)
-%_cpp.v: %.cpp $(CPP2V)
-	$(CPP2V) -o $@ $< -- $(CFLAGS)
-%_hpp.v: %.hpp $(CPP2V)
-	$(CPP2V) -o $@ $< -- $(CFLAGS)
-
-%_c_spec.v: %.c $(CPP2V)
-	$(CPP2V) -spec $@ $< -- $(CFLAGS)
-%_h_spec.v: %.h $(CPP2V)
-	$(CPP2V) -spec $@ $< -- $(CFLAGS)
-%_cpp_spec.v: %.cpp $(CPP2V)
-	$(CPP2V) -spec $@ $< -- $(CFLAGS)
-%_hpp_spec.v: %.hpp $(CPP2V)
-	$(CPP2V) -spec $@ $< -- $(CFLAGS)
-
-%.o: %.cpp
-	gcc -c $<
+	@ $(MAKE) -f Makefile.coq clean
+	rm -f Makefile.coq
 
 Makefile.coq: $(VS)
 	coq_makefile -f _CoqProject -o Makefile.coq
